Cleanup definitions related to the discussion in the meeting.
SimulationLayer.v contains the minimal required definitions.

src/LayerTransfer.v
@@ -10,8 +10,8 @@ Section LayerTransfer.
 
   Definition right_total_filtered {T1 T2: Type} (R: T1 -> T2 -> Prop) (P: T2 -> Prop):=
     forall t2,
-    P t2 ->
-    exists t1, R t1 t2.
+      P t2 ->
+      exists t1, R t1 t2.
 
   Definition refines_to (s1 s2: state) :=
     Prog.get_user s1 = get_user s2 /\
@@ -21,9 +21,9 @@ Section LayerTransfer.
 
   Ltac simpl_refines_to :=
     unfold refines_to, Prog.get_user, get_user,
-        Prog.get_oracle, get_oracle,
-        Prog.get_disk, get_disk,
-        Prog.get_store, get_store in *; simpl in *.
+    Prog.get_oracle, get_oracle,
+    Prog.get_disk, get_disk,
+    Prog.get_store, get_store in *; simpl in *.
 
   
   Ltac simpl_states:=
@@ -31,140 +31,141 @@ Section LayerTransfer.
 
   Definition refines_to_same st1 st2 := exists sr, refines_to st1 sr /\ refines_to st2 sr.
 
+  Definition refines_to_related R st1 st2 := exists sr1 sr2, refines_to st1 sr1 /\ refines_to st2 sr2 /\ R sr1 sr2.
 
   Lemma exec_preserves_user:
-      forall T (p: prog T) st1 st1' tr,
-        exec st1 p st1' tr ->
-        Prog.get_user st1 = Prog.get_user (extract_state st1').
-    Proof.
-      induction 1; simpl in *; eauto.
-      cleanup; eauto.
-    Qed.
+    forall T (p: prog T) st1 st1' tr,
+      exec st1 p st1' tr ->
+      Prog.get_user st1 = Prog.get_user (extract_state st1').
+  Proof.
+    induction 1; simpl in *; eauto.
+    cleanup; eauto.
+  Qed.
 
-    Lemma exec_limited_preserves_user:
-      forall T (p: prog_limited T) st1 st1',
-        exec_limited st1 p st1' ->
-        Prog.get_user st1 = Prog.get_user (extract_state st1').
-    Proof.
-      induction 1; simpl in *; eauto.
-      eapply exec_preserves_user; eauto.
-    Qed.
+  Lemma exec_limited_preserves_user:
+    forall T (p: prog_limited T) st1 st1',
+      exec_limited st1 p st1' ->
+      Prog.get_user st1 = Prog.get_user (extract_state st1').
+  Proof.
+    induction 1; simpl in *; eauto.
+    eapply exec_preserves_user; eauto.
+  Qed.
 
-    Lemma rep_equivalent_for_fst_low:
-      forall u d1 d2 d1' d2',
-        @equivalent_for_fst _ addr_dec _ u d1 d1' ->
-        rep d2 d1 ->
-        rep d2' d1' ->
-        @equivalent_for_fst _ addr_dec _ u d2 d2'.
-    Proof.
-      unfold equivalent_for, equivalent_for_fst, rep; intros.
-      destruct_lift H0; destruct_lift H1; cleanup.
+  Lemma rep_equivalent_for_fst_low:
+    forall u d1 d2 d1' d2',
+      @equivalent_for_fst _ addr_dec _ u d1 d1' ->
+      rep d2 d1 ->
+      rep d2' d1' ->
+      @equivalent_for_fst _ addr_dec _ u d2 d2'.
+  Proof.
+    unfold equivalent_for, equivalent_for_fst, rep; intros.
+    destruct_lift H0; destruct_lift H1; cleanup.
 
-      specialize (H 0) as Hx; destruct Hx; cleanup.
-      erewrite ptsto_valid in H2; [| pred_apply; cancel]; cleanup.
-      
-      erewrite ptsto_valid in H2; [| pred_apply; cancel]; cleanup.
-      erewrite ptsto_valid in H3; [| pred_apply; cancel]; cleanup.
-      simpl in *; cleanup.
-      specialize (H18 (can_access_public u)); inversion H18; cleanup.
-
-      specialize (H a) as Hx.
-      
-      destruct (Compare_dec.le_lt_dec a 2); [|intuition].
-      destruct a; [intuition|].
-      destruct a.
-      destruct Hx; cleanup.
-      erewrite ptsto_valid in H2; [| pred_apply; cancel]; cleanup.
-      
-      erewrite ptsto_valid in H2; [| pred_apply; cancel]; cleanup.
-      erewrite ptsto_valid in H3; [| pred_apply; cancel]; cleanup.
-      simpl in *; cleanup.      
-      
-      destruct (value_to_nat dummy1); [intuition|].
-      destruct n; [intuition|].
-      right; do 2 eexists; intuition eauto; simpl in *.
-      destruct n; [intuition|].
-      destruct n; [intuition|].
-      right; do 2 eexists; intuition eauto; simpl in *.
-      omega.
-
-                             destruct a; [|intuition].
-      destruct Hx; cleanup.
-      erewrite ptsto_valid in H2; [| pred_apply; cancel]; cleanup.
-      
-      erewrite ptsto_valid in H2; [| pred_apply; cancel]; cleanup.
-      erewrite ptsto_valid in H3; [| pred_apply; cancel]; cleanup.
-      simpl in *; cleanup.      
-      
-      destruct (value_to_nat dummy1); [intuition|].
-      destruct n; [intuition|].
-      destruct n; [intuition|].
-      right; do 2 eexists; intuition eauto; simpl in *.
-      destruct n; [intuition|].
-      right; do 2 eexists; intuition eauto; simpl in *.
-      omega.
-    Qed.
-
+    specialize (H 0) as Hx; destruct Hx; cleanup.
+    erewrite ptsto_valid in H2; [| pred_apply; cancel]; cleanup.
     
-    Lemma exec_limited_preserves_rep:
-      forall T (p: prog_limited T)  st1 d1 st1',
-        exec_limited st1 p st1' ->
-        rep d1 (Prog.get_disk st1) ->
-        exists d1', rep d1' (Prog.get_disk (extract_state st1')).
-    Proof.
-      induction p; intros; cleanup; simpl in *; eauto;
-        unfold Prog.get_disk, state in *; destruct_pairs; simpl in *;
-      try (inversion H; sigT_eq); simpl in *.
-      - edestruct alloc_ok; eauto.
-        apply pimpl_star_emp; eauto.       
-        destruct H1; cleanup;
-        destruct_lift H3; eauto.
+    erewrite ptsto_valid in H2; [| pred_apply; cancel]; cleanup.
+    erewrite ptsto_valid in H3; [| pred_apply; cancel]; cleanup.
+    simpl in *; cleanup.
+    specialize (H18 (can_access_public u)); inversion H18; cleanup.
 
-      - edestruct free_ok; eauto.
-        apply pimpl_star_emp; eauto.
-        destruct H1; cleanup;
-        destruct_lift H3; eauto.
-
-      - edestruct read_ok; eauto.
-        apply pimpl_star_emp; eauto.
-        destruct H1; cleanup;
-        destruct_lift H3; eauto.
-
-      - edestruct write_ok'; eauto.
-        apply pimpl_star_emp; eauto.
-        destruct H1; cleanup;
-          destruct_lift H3; eauto.
-        
-      - invert_exec; cleanup; simpl in *; eauto.
-
-      - inversion H0; sigT_eq; simpl in *.
-        invert_exec.
-        edestruct IHp; eauto; cleanup; simpl in *.
-        econstructor; eauto.
-        simpl; eauto.
-        simpl in *.
-
-        edestruct H; eauto; cleanup; simpl in *.
-        econstructor; eauto.
-        simpl; eauto.
-        
-        destruct H6; cleanup; simpl in *.
-        edestruct IHp; eauto; cleanup; simpl in *.
-        econstructor; eauto.
-        simpl; eauto.
-        simpl; eauto.
-
-        edestruct IHp; eauto; cleanup; simpl in *.
-        econstructor; eauto.
-        simpl; eauto.
-        simpl in *.
-
-        edestruct H; eauto; cleanup; simpl in *.
-        econstructor; eauto.
-        simpl; eauto.
-    Qed.
-
+    specialize (H a) as Hx.
     
+    destruct (Compare_dec.le_lt_dec a 2); [|intuition].
+    destruct a; [intuition|].
+    destruct a.
+    destruct Hx; cleanup.
+    erewrite ptsto_valid in H2; [| pred_apply; cancel]; cleanup.
+    
+    erewrite ptsto_valid in H2; [| pred_apply; cancel]; cleanup.
+    erewrite ptsto_valid in H3; [| pred_apply; cancel]; cleanup.
+    simpl in *; cleanup.      
+    
+    destruct (value_to_nat dummy1); [intuition|].
+    destruct n; [intuition|].
+    right; do 2 eexists; intuition eauto; simpl in *.
+    destruct n; [intuition|].
+    destruct n; [intuition|].
+    right; do 2 eexists; intuition eauto; simpl in *.
+    omega.
+
+    destruct a; [|intuition].
+    destruct Hx; cleanup.
+    erewrite ptsto_valid in H2; [| pred_apply; cancel]; cleanup.
+    
+    erewrite ptsto_valid in H2; [| pred_apply; cancel]; cleanup.
+    erewrite ptsto_valid in H3; [| pred_apply; cancel]; cleanup.
+    simpl in *; cleanup.      
+    
+    destruct (value_to_nat dummy1); [intuition|].
+    destruct n; [intuition|].
+    destruct n; [intuition|].
+    right; do 2 eexists; intuition eauto; simpl in *.
+    destruct n; [intuition|].
+    right; do 2 eexists; intuition eauto; simpl in *.
+    omega.
+  Qed.
+
+  
+  Lemma exec_limited_preserves_rep:
+    forall T (p: prog_limited T)  st1 d1 st1',
+      exec_limited st1 p st1' ->
+      rep d1 (Prog.get_disk st1) ->
+      exists d1', rep d1' (Prog.get_disk (extract_state st1')).
+  Proof.
+    induction p; intros; cleanup; simpl in *; eauto;
+      unfold Prog.get_disk, state in *; destruct_pairs; simpl in *;
+        try (inversion H; sigT_eq); simpl in *.
+    - edestruct alloc_ok; eauto.
+      apply pimpl_star_emp; eauto.       
+      destruct H1; cleanup;
+        destruct_lift H3; eauto.
+
+    - edestruct free_ok; eauto.
+      apply pimpl_star_emp; eauto.
+      destruct H1; cleanup;
+        destruct_lift H3; eauto.
+
+    - edestruct read_ok; eauto.
+      apply pimpl_star_emp; eauto.
+      destruct H1; cleanup;
+        destruct_lift H3; eauto.
+
+    - edestruct write_ok'; eauto.
+      apply pimpl_star_emp; eauto.
+      destruct H1; cleanup;
+        destruct_lift H3; eauto.
+      
+    - invert_exec; cleanup; simpl in *; eauto.
+
+    - inversion H0; sigT_eq; simpl in *.
+      invert_exec.
+      edestruct IHp; eauto; cleanup; simpl in *.
+      econstructor; eauto.
+      simpl; eauto.
+      simpl in *.
+
+      edestruct H; eauto; cleanup; simpl in *.
+      econstructor; eauto.
+      simpl; eauto.
+      
+      destruct H6; cleanup; simpl in *.
+      edestruct IHp; eauto; cleanup; simpl in *.
+      econstructor; eauto.
+      simpl; eauto.
+      simpl; eauto.
+
+      edestruct IHp; eauto; cleanup; simpl in *.
+      econstructor; eauto.
+      simpl; eauto.
+      simpl in *.
+
+      edestruct H; eauto; cleanup; simpl in *.
+      econstructor; eauto.
+      simpl; eauto.
+  Qed.
+
+  
 
   Definition prog_eq T (p1: Op prog_limited_LTS T) (p2: Op prog2_LTS T) := p1 = p2.
 
@@ -172,10 +173,10 @@ Section LayerTransfer.
   Definition something_refines_to st2 := exists st1, refines_to st1 st2.
 
   Lemma exec_limited_preserves_refines_to_something:
-      forall T (p: prog_limited T)  st1 st1',
-        exec_limited st1 p st1' ->
-        refines_to_something st1 ->
-        refines_to_something (extract_state st1').
+    forall T (p: prog_limited T)  st1 st1',
+      exec_limited st1 p st1' ->
+      refines_to_something st1 ->
+      refines_to_something (extract_state st1').
   Proof.
     unfold refines_to_something; intros.
     simpl_refines_to; simpl_states; cleanup.
@@ -185,7 +186,27 @@ Section LayerTransfer.
     exists(fst (fst (fst (extract_state st1'))), snd (fst (fst (extract_state st1'))), x, snd (extract_state st1'));
       intuition eauto.
   Qed.
-
+  
+  (*
+  Lemma exec2_preserves_refines_to_something:
+      forall T (p: prog_limited T)  st1 st1',
+        exec2 st1 p st1' ->
+        refines_to_something st1 ->
+        refines_to_something (extract_state st1').
+  Proof.
+    unfold refines_to_something; intros.
+    inversion H; sigT_eq; simpl in *; cleanup.
+    eapply exec_limited_preserves_refines_to_something in H3; eauto.
+    unfold refines_to_something in *; 
+    simpl_refines_to; simpl_states; cleanup.
+    eapply exec_limited_preserves_rep in H; eauto; cleanup.
+    unfold get_disk in *.
+    simpl_states; cleanup.
+    exists(fst (fst (fst (extract_state st1'))), snd (fst (fst (extract_state st1'))), x, snd (extract_state st1'));
+      intuition eauto.
+  Qed.
+   *)
+  
   Lemma return_state_equivalent_for_refines_to:
     forall T u (x y a b: @Result state T),
       refines_to (extract_state x) (extract_state y) ->
@@ -226,195 +247,148 @@ Section LayerTransfer.
     eapply rep_equivalent_for_fst_low; eauto.
   Qed.
 
-(*
-  Theorem transfer_low_to_high_self :
-  forall T (p: prog_limited T) valid_l valid_h refines_to,
-  data_noninterference p valid_l ->
-  StrongBisimulation prog_limited_LTS prog2_LTS prog_eq refines_to ->
-  (forall u, simulation_preserving (Prog.state_equivalent_for u) (state_equivalent_for u) refines_to) ->
-  data_noninterference p valid_h.
-Proof.
-  unfold something_refines_to, refines_to_something, simulation_preserving, result_same, prog_eq; intros.
-  destruct H, H0.
-  rename H1 into simulation_preserving.
+  Definition simulation_preserving_right_to_left {T1 T2: Type} (S1: T1 -> T1 -> Prop) (S2: T2 -> T2 -> Prop)(R: T1 -> T2 -> Prop) :=
+    forall t1 t1' t2 t2',
+      R t1 t2 ->
+      R t1' t2' ->
+      S2 t2 t2' -> S1 t1 t1'.
 
-  unfold data_noninterference; split.
-  - unfold state_noninterference; intros.
-    destruct 
-    eapply_fresh strong_bisimulation_correct in H3; eauto; cleanup; simpl in *.
+  Definition simulation_preserving_left_to_right {T1 T2: Type} (S1: T1 -> T1 -> Prop) (S2: T2 -> T2 -> Prop)(R: T1 -> T2 -> Prop) :=
+    forall t1 t1' t2 t2',
+      R t1 t2 ->
+      R t1' t2' ->
+      S1 t1 t1' -> S2 t2 t2'.
 
-    eapply_fresh H in H3 cleanup.
-    simpl_refines_to; simpl_states; cleanup; eauto.
-    eapply_fresh strong_bisimulation_correct0 in H6; eauto; cleanup; simpl in *.
-    edestruct H9; [econstructor; eauto|]; cleanup.
-    eexists; intuition eauto.
+  Lemma test:
+    (forall T (p: prog_limited T), ProgLimited.data_noninterference p refines_to_something) ->
     
-    unfold return_state_equivalent_for.
-    unfold result_same in *; cleanup; intuition eauto;
-    simpl in *;
-    unfold state_equivalent_for, Prog.state_equivalent_for in *; cleanup;
-    unfold RS in *; simpl in *;
-    unfold state, state2 in *; destruct_pairs; simpl in *; cleanup;
-    unfold Prog.get_user, get_user,
-    Prog.get_oracle, get_oracle,
-    Prog.get_disk, get_disk in *; simpl in *; cleanup;
-    intuition eauto; eapply rep_equivalent_for; eauto.
+    (forall u, SelfSimulation prog_limited_LTS (refines_to_related (state_equivalent_for u))).
+  Proof.
+    intros; constructor; intros; simpl in *.
+    specialize (H T o).
+    unfold refines_to_related in *; cleanup.
+    destruct H.
+    eapply_fresh H in H0.
+    all: unfold refines_to_something; eauto.
+    eapply_fresh H4 in H0.
+    all: unfold refines_to_something; eauto.
+    simpl in *; eauto; cleanup.
+    eexists; intuition eauto.
+  Abort.
 
-    unfold RS in H5; cleanup; eauto.
-    eapply simulation_preserving; eauto.
-
-  -  unfold ret_noninterference; intros.
-     edestruct (right_total_state st1), (right_total_state st2); eauto.
-     edestruct (right_total_op T p).
-     eapply_fresh strong_bisimulation_correct0 in H5; eauto; cleanup; simpl in *.
-     apply H9 in H2; cleanup; clear H8 H9.
-     
-     inversion H2; sigT_eq.
-     unfold RP in *; cleanup.
-     unfold Prog.state_noninterference, Prog.ret_noninterference in *.
-     eapply_fresh H4 in H15; eauto; cleanup.
-     eapply_fresh strong_bisimulation_correct0 in H6; eauto; cleanup; simpl in *.     
-     edestruct H9; [econstructor; eauto|]; cleanup.
-     eexists; intuition eauto.
-     
-     unfold return_equivalent_for.
-     unfold result_same in *; cleanup; intuition eauto;
-       simpl in *;
-       unfold state_equivalent_for, Prog.state_equivalent_for in *; cleanup;
-         unfold RS in *; simpl in *;
-           unfold state, state2 in *; destruct_pairs; simpl in *; cleanup;
-             unfold Prog.get_user, get_user,
-             Prog.get_oracle, get_oracle,
-             Prog.get_disk, get_disk in *; simpl in *; cleanup;
-               intuition eauto; try eapply rep_equivalent_for; eauto.
-     
-     cleanup; eauto.
-     unfold RS in H5; simpl in *; cleanup; eauto.
-     pose proof H5 as Hx; unfold RS in H5; simpl in *; cleanup; eauto.
-     eapply simulation_preserving; eauto.
-Qed.
-
-
-*)
-
-
-Definition simulation_preserving_right_to_left {T1 T2: Type} (S1: T1 -> T1 -> Prop) (S2: T2 -> T2 -> Prop)(R: T1 -> T2 -> Prop) :=
-  forall t1 t1' t2 t2',
-    R t1 t2 ->
-    R t1' t2' ->
-    S2 t2 t2' -> S1 t1 t1'.
-
-Lemma test:
-  (forall u, SelfSimulation prog_limited_LTS (Prog.state_equivalent_for u)) ->
-  SelfSimulation prog_limited_LTS refines_to_same.
-Proof.
-  intros; constructor; intros; simpl in *.
-  eapply_fresh H in H0.
-  simpl in *; eauto; cleanup.
-  eexists; intuition eauto.
-Abort.
   
 
   Theorem transfer_low_to_high_self :
-  forall T (p: prog_limited T),
-  ProgLimited.data_noninterference p refines_to_something ->
-  StrongBisimulation prog_limited_LTS prog2_LTS prog_eq refines_to ->
-  (forall u, simulation_preserving_right_to_left (Prog.state_equivalent_for u) (state_equivalent_for u) refines_to) ->
-  data_noninterference p something_refines_to.
-Proof.
-  unfold something_refines_to, refines_to_something, simulation_preserving_right_to_left, result_same, prog_eq; intros.
-  destruct H, H0.
-  rename H1 into simulation_preserving.
+    forall T (p: prog_limited T),
+      (forall u, SelfSimulation prog_limited_LTS (refines_to_related (state_equivalent_for u))) ->
+      StrongBisimulation prog_limited_LTS prog2_LTS prog_eq refines_to ->
+      data_noninterference p something_refines_to.
+  Proof.
+    unfold something_refines_to, refines_to_something, simulation_preserving_right_to_left, result_same, prog_eq; intros.
+    destruct H0.
 
-  unfold data_noninterference; split.
-  - unfold state_noninterference; intros; cleanup.
-    eapply_fresh strong_bisimulation_correct in H3; eauto; cleanup; simpl in *.
-
-    edestruct H.
-    eexists; apply H0.
-    eexists; apply H1.
-    eauto.
-
-    (* eq_h -> eq_l required here *)
-    eapply simulation_preserving; eauto.
-    cleanup.
-
-    (* exec_limited preserves refines_to_something required in here *)
-    eapply_fresh exec_limited_preserves_refines_to_something in H9; unfold refines_to_something in *;
-      eauto; cleanup.
-    eapply_fresh exec_limited_preserves_user in H9; unfold get_user in *; simpl in *; cleanup.
-                                                                                  
-    destruct x2.
-    + simpl_states; cleanup; eauto.
-      eexists; split.
-      simpl_refines_to; cleanup.
-      econstructor; eauto.
-      simpl_refines_to; cleanup.
-      eapply return_state_equivalent_for_refines_to; eauto;
-        simpl_refines_to; intuition eauto.
+    unfold data_noninterference; split.
+    - unfold state_noninterference; intros; cleanup.
+      specialize (H viewer).
+      destruct H.
+      eapply_fresh strong_bisimulation_correct in H2; eauto; cleanup; simpl in *.
+      eapply_fresh self_simulation_correct in H; eauto; cleanup; simpl in *.
+      2: {
+        unfold refines_to_related.
+        do 2 eexists; eauto.
+      }
       
-    + simpl_states; cleanup; eauto.
-      eexists; split.
-      simpl_refines_to; cleanup.
-      eapply Exec2Crashed; eauto.
-      simpl_refines_to; cleanup.
-      eapply return_state_equivalent_for_refines_to; eauto;
-        simpl_refines_to; intuition eauto.
-
-  - unfold ret_noninterference; intros; cleanup.
-    eapply_fresh strong_bisimulation_correct in H3; eauto; cleanup; simpl in *.
-
-    edestruct H2.
-    eexists; apply H0.
-    eexists; apply H1.
-    eauto.
-    
-    (* eq_h -> eq_l required here *)
-    eapply simulation_preserving; eauto.
-    simpl_refines_to; cleanup; eauto.
-    cleanup.
-
-    (* exec_limited preserves refines_to_something required in here *)
-    eapply_fresh exec_limited_preserves_refines_to_something in H9; unfold refines_to_something in *;
-      eauto; cleanup.
-    eapply_fresh exec_limited_preserves_user in H9; unfold get_user in *; simpl in *; cleanup.
-                                                                                  
-    destruct x2.
-    + simpl_states; cleanup; eauto.
-      eexists; split.
-      simpl_refines_to; cleanup.
-      econstructor; eauto.
-      eapply return_equivalent_for_refines_to.
-      6: simpl_refines_to; cleanup; eauto.
-      all: simpl; eauto.
-      simpl_refines_to; cleanup; intuition eauto.
+      (* exec_limited preserves refines_to_something required in here *)
+      eapply_fresh exec_limited_preserves_user in H7; unfold get_user in *; simpl in *; cleanup.
+      unfold refines_to_related in *; cleanup.
       
-    + simpl_states; cleanup; eauto.
-      eexists; split.
-      simpl_refines_to; cleanup.
-      eapply Exec2Crashed; eauto.
-      eapply return_equivalent_for_refines_to.
-      6: simpl_refines_to; cleanup; eauto.
-      all: simpl; eauto.
-      simpl_refines_to; cleanup; intuition eauto.
-Qed.  
+      destruct x2.
+      + simpl_states; cleanup; eauto.
+        eexists; split.
+        simpl_refines_to; cleanup.
+        rewrite e5 in *.
+        econstructor; eauto.
+        unfold result_same in *; cleanup; intuition; simpl in *.
+        simpl_refines_to; cleanup.
+        intuition; cleanup.
+        simpl_states; cleanup. intuition eauto.
+
+        (* rep equivalent_for_fst relation *)
+        admit.
+        
+        
+      + simpl_states; cleanup; eauto.
+        eexists; split.
+        simpl_refines_to; cleanup.
+        rewrite e5 in *.
+        eapply Exec2Crashed; eauto.
+        simpl_refines_to; cleanup.
+        unfold result_same in *; cleanup; intuition; simpl in *.
+        simpl_refines_to; cleanup.
+        intuition; cleanup.
+        simpl_states; cleanup. intuition eauto.
+
+        (* rep equivalent_for_fst relation *)
+        admit. 
+
+    - unfold ret_noninterference; intros; cleanup.
+      specialize (H (get_user st1)).
+      destruct H.
+      eapply_fresh strong_bisimulation_correct in H2; eauto; cleanup; simpl in *.
+
+      eapply_fresh self_simulation_correct in H; eauto; cleanup; simpl in *.
+      2: {
+        unfold refines_to_related.
+        do 2 eexists; eauto.
+      }
+      
+
+      (* exec_limited preserves refines_to_something required in here *)
+      eapply_fresh exec_limited_preserves_user in H7; unfold get_user in *; simpl in *; cleanup.
+      unfold refines_to_related in *; cleanup.
+      
+      destruct x2.
+      + simpl_states; cleanup; eauto.
+        eexists; split.
+        simpl_refines_to; cleanup.
+        rewrite e5 in *.
+        econstructor; eauto.
+        unfold result_same in *; cleanup; intuition; simpl in *.
+        simpl_refines_to; cleanup.
+        intuition; cleanup; eauto.
+        simpl_states; cleanup. intuition eauto.
+        (* rep equivalent_for_fst relation *)
+        admit. 
+        
+      + simpl_states; cleanup; eauto.
+        eexists; split.
+        simpl_refines_to; cleanup.
+        rewrite e5 in *.
+        eapply Exec2Crashed; eauto.
+        unfold result_same in *; cleanup; intuition; simpl in *.
+        simpl_refines_to; cleanup.
+        intuition; cleanup; eauto.
+        simpl_states; cleanup; intuition eauto.
+        (* rep equivalent_for_fst relation *)
+        admit. 
+  Admitted.  
 
 
-Lemma exec_limited_preserves_refinement:
-      forall T (p: prog_limited T)  st1 st2 st1',
-        exec_limited st1 p st1' ->
-        refines_to_same st1 st2 ->
-        exists st2',
-          exec_limited st2 p st2' /\
-          result_same st1' st2' /\
-          refines_to_same (extract_state st1') (extract_state st2') /\
-          (forall def : T, extract_ret def st1' = extract_ret def st2').
+  Lemma exec_limited_preserves_refinement:
+    forall T (p: prog_limited T)  st1 st2 st1',
+      exec_limited st1 p st1' ->
+      refines_to_same st1 st2 ->
+      exists st2',
+        exec_limited st2 p st2' /\
+        result_same st1' st2' /\
+        refines_to_same (extract_state st1') (extract_state st2') /\
+        (forall def : T, extract_ret def st1' = extract_ret def st2').
   Proof.
     unfold refines_to_same; induction p; simpl in *;
-        intros; cleanup.
+      intros; cleanup.
     
     - inversion H; sigT_eq; clear H;
-          simpl_states.
+        simpl_states.
       edestruct alloc_ok; eauto.
       apply pimpl_star_emp; eauto.
       simpl_refines_to; cleanup; eauto.
@@ -422,7 +396,7 @@ Lemma exec_limited_preserves_refinement:
       destruct H; cleanup; destruct_lifts.
       + destruct H7; cleanup.
         simpl_refines_to; cleanup.
-      (* needs complete correctness *)
+        (* needs complete correctness *)
   Admitted.
 
   Lemma rep_trans:
@@ -439,97 +413,97 @@ Lemma exec_limited_preserves_refinement:
   Admitted.
 
   Theorem RS_strong_bisimulation:
-      StrongBisimulation prog_limited_LTS prog2_LTS prog_eq refines_to.
-    Proof.
-      unfold prog_eq; constructor; intros.
-      cleanup; simpl in *.
-      split; intros.
+    StrongBisimulation prog_limited_LTS prog2_LTS prog_eq refines_to.
+  Proof.
+    unfold prog_eq; constructor; intros.
+    cleanup; simpl in *.
+    split; intros.
 
-      - eapply_fresh exec_limited_preserves_rep in H; cleanup; simpl in *; eauto.
-        eapply_fresh exec_limited_preserves_user in H; simpl in *; cleanup.
-        destruct s1'; simpl_refines_to; simpl_states; cleanup.
-        eexists; intuition.
-        econstructor; eauto.
-        all: simpl; eauto.
-        
-        eexists; intuition.
-        eapply Exec2Crashed; simpl; eauto.
-        all: simpl; eauto.
+    - eapply_fresh exec_limited_preserves_rep in H; cleanup; simpl in *; eauto.
+      eapply_fresh exec_limited_preserves_user in H; simpl in *; cleanup.
+      destruct s1'; simpl_refines_to; simpl_states; cleanup.
+      eexists; intuition.
+      econstructor; eauto.
+      all: simpl; eauto.
+      
+      eexists; intuition.
+      eapply Exec2Crashed; simpl; eauto.
+      all: simpl; eauto.
 
-        simpl_refines_to; cleanup; eauto.
-        
-      - inversion H; sigT_eq; clear H.
-        simpl_refines_to; simpl_states; cleanup.
-        eapply exec_limited_preserves_refinement in H3; unfold refines_to_same in *;
+      simpl_refines_to; cleanup; eauto.
+      
+    - inversion H; sigT_eq; clear H.
+      simpl_refines_to; simpl_states; cleanup.
+      eapply exec_limited_preserves_refinement in H3; unfold refines_to_same in *;
         simpl in *; cleanup.
-        2: {
-          exists(u,o,dh,s); split.
-          simpl_refines_to; intuition.
-          instantiate (1:= (u, o, x1, s)).
-          simpl_refines_to; intuition eauto.
-        }
-        
-        simpl_refines_to; cleanup; intuition.
-        eexists; intuition.
+      2: {
+        exists(u,o,dh,s); split.
+        simpl_refines_to; intuition.
+        instantiate (1:= (u, o, x1, s)).
+        simpl_refines_to; intuition eauto.
+      }
+      
+      simpl_refines_to; cleanup; intuition.
+      eexists; intuition.
+      eauto.
+      all: simpl in *; eauto.
+      eapply rep_trans; eauto.
+
+      eapply exec_limited_preserves_refinement in H3; unfold refines_to_same in *;
+        simpl in *; cleanup.
+      2: {
+        exists(u,o,dh,s); split.
+        simpl_refines_to; intuition.
         eauto.
-        all: simpl in *; eauto.
-        eapply rep_trans; eauto.
-
-        eapply exec_limited_preserves_refinement in H3; unfold refines_to_same in *;
-          simpl in *; cleanup.
-         2: {
-          exists(u,o,dh,s); split.
-          simpl_refines_to; intuition.
-          eauto.
-        }
-        simpl_refines_to; cleanup; intuition.
-        eexists; intuition.
-        eauto.
-        all: simpl in *; eauto.
-        eapply rep_trans; eauto.
-    Qed.
+      }
+      simpl_refines_to; cleanup; intuition.
+      eexists; intuition.
+      eauto.
+      all: simpl in *; eauto.
+      eapply rep_trans; eauto.
+  Qed.
 
 
 
 
 
-    Lemma exec_deterministic_oracle:
-      forall T (p: prog T) st1 st2 st1' st2' tr1 tr2,
-        exec st1 p st1' tr1 ->
-        exec st2 p st2' tr2 ->
-        Prog.get_oracle st1 = Prog.get_oracle st2 ->
-        Prog.get_oracle (extract_state st1') = Prog.get_oracle (extract_state st2').
-    Proof.
-      unfold Prog.get_oracle;
-        induction p; intros; simpl in *;
-          simpl_states; cleanup;
-            invert_exec; invert_exec;
-              cleanup; simpl in *;
-          cleanup; eauto;
-      try match goal with
-      |[H: _ :: _ = _ :: _ |- _] =>
-       inversion H; eauto
-      end.      
-      simpl_states; cleanup.
-   Abort.
+  Lemma exec_deterministic_oracle:
+    forall T (p: prog T) st1 st2 st1' st2' tr1 tr2,
+      exec st1 p st1' tr1 ->
+      exec st2 p st2' tr2 ->
+      Prog.get_oracle st1 = Prog.get_oracle st2 ->
+      Prog.get_oracle (extract_state st1') = Prog.get_oracle (extract_state st2').
+  Proof.
+    unfold Prog.get_oracle;
+      induction p; intros; simpl in *;
+        simpl_states; cleanup;
+          invert_exec; invert_exec;
+            cleanup; simpl in *;
+              cleanup; eauto;
+                try match goal with
+                    |[H: _ :: _ = _ :: _ |- _] =>
+                     inversion H; eauto
+                    end.      
+    simpl_states; cleanup.
+  Abort.
 
 
-    
-    
+  
+  
 
-   
+  
 
 
 
-    
+  
   
   
   
 
-    
-    
-    
-                                     (*
+  
+  
+  
+  (*
     Lemma rep_equivalent_for_fst_high:
       forall u d1 d2 d1' d2',
         @equivalent_for_fst _ addr_dec _ u d2 d2' ->
@@ -612,4 +586,4 @@ Lemma exec_limited_preserves_refinement:
       omega.
     Qed.
 
-*)
+   *)
