src/SimulationLayer.v
@@ -1,0 +1,145 @@
+Require Import List.
+
+Inductive Result {State T: Type} :=
+| Finished : State -> T -> @Result State T
+| Crashed : State -> @Result State T.
+
+Definition extract_state {State T} (res: @Result State T) :=
+  match res with
+  | Finished s _ | Crashed s => s
+  end.
+
+Definition extract_ret {State T} def (res: @Result State T) :=
+  match res with
+  | Finished _ r => r
+  | Crashed _ => def
+  end.
+
+Definition result_same {State1 State2 T1 T2} (res1: @Result State1 T1) (res2: @Result State2 T2) :=
+  match res1, res2 with
+  | Finished _ _, Finished _ _ | Crashed _, Crashed _ => True
+  | _, _ => False
+  end.
+
+Lemma result_same_transitive:
+  forall State1 State2 State3 T1 T2 T3
+    (res1: @Result State1 T1)
+    (res2: @Result State2 T2)
+    (res3: @Result State3 T3),
+    result_same res1 res2 ->
+    result_same res2 res3 ->
+    result_same res1 res3.
+Proof.
+  unfold result_same; intros.
+  destruct res1, res2, res3; intuition.
+Qed.
+
+Lemma result_same_symmetric:
+  forall State1 State2 T1 T2
+    (res1: @Result State1 T1)
+    (res2: @Result State2 T2),
+    result_same res1 res2 ->
+    result_same res2 res1.
+Proof.
+  unfold result_same; intros.
+  destruct res1, res2; intuition.
+Qed.
+
+Record LTS :=
+  {
+    State : Type;
+    Op : Type -> Type;
+    transition : forall T, State -> Op T -> @Result State T -> Prop;
+  }.
+
+Record SelfSimulation (lts: LTS) (R: State lts -> State lts -> Prop):=
+  {
+    self_simulation_correct:
+      forall T o s1 s1' s2,
+        (transition lts) T s1 o s1' ->
+        R s1 s2 ->
+        exists s2',
+          (transition lts) T s2 o s2' /\
+          result_same s1' s2' /\
+          R (extract_state s1') (extract_state s2') /\
+          (forall def, extract_ret def s1' = extract_ret def s2');
+  }.
+
+Record StrongBisimulation  (lts1 lts2 : LTS) (compile: forall T, Op lts2 T -> Op lts1 T) (refines_to: State lts1 -> State lts2 -> Prop):=
+  {
+    strong_bisimulation_correct:
+      (forall T o2 s1 s2,
+          refines_to s1 s2 ->
+          (forall s1',
+              (transition lts1) T s1 (compile T o2) s1' ->
+              exists s2',
+                (transition lts2) T s2 o2 s2' /\
+                result_same s1' s2' /\
+                refines_to (extract_state s1') (extract_state s2') /\
+                (forall def, extract_ret def s1' = extract_ret def s2')) /\
+          (forall s2',
+              (transition lts2) T s2 o2 s2' ->
+              exists s1',
+                (transition lts1) T s1 (compile T o2) s1' /\
+                result_same s1' s2' /\
+                refines_to (extract_state s1') (extract_state s2') /\
+                (forall def, extract_ret def s1' = extract_ret def s2')))
+  }.
+
+
+
+Definition right_total {T1 T2: Type} (R: T1 -> T2 -> Prop) :=
+  forall t2, exists t1, R t1 t2.
+
+Definition refines_to_related {T1 T2} refines_to eqv_h (st1 st2: T1) :=
+  exists (sr1 sr2: T2),
+    refines_to st1 sr1 /\
+    refines_to st2 sr2 /\
+    eqv_h sr1 sr2.
+
+Definition deterministic_refinement {T1 T2} refines_to eqv_h :=
+  forall (s:T1) (sr1 sr2: T2),
+    refines_to s sr1 ->
+    refines_to s sr2 ->
+    eqv_h sr1 sr2.
+
+Definition transitive {T} (R: T -> T -> Prop) :=
+  forall t t' t'', R t t' -> R t' t'' -> R t t''.
+
+
+
+
+Theorem transfer_low_to_high :
+  forall low high eqv_h refines_to compile,
+    SelfSimulation low (refines_to_related refines_to eqv_h) ->
+    StrongBisimulation low high compile refines_to ->
+    right_total refines_to ->
+    deterministic_refinement refines_to eqv_h ->
+    transitive eqv_h ->
+    SelfSimulation high eqv_h.
+Proof.
+  unfold right_total, refines_to_related, deterministic_refinement; intros.
+  destruct H, H0.
+  rename self_simulation_correct0 into self_simulation_correct.
+  rename H1 into right_total_state.
+  rename strong_bisimulation_correct0 into strong_bisimulation_correct.
+  
+  eapply Build_SelfSimulation;  intros.
+  edestruct (right_total_state s1), (right_total_state s2).
+  eapply strong_bisimulation_correct in H1 as Hx; destruct Hx.
+  apply H6 in H.
+  repeat destruct H. destruct H7, H8.
+  
+  eapply self_simulation_correct in H; eauto; repeat destruct H. destruct H10, H11.
+  repeat destruct H11.
+  destruct H13.
+  
+  eapply strong_bisimulation_correct in H4 as Hx; destruct Hx.
+  apply H15 in H.
+  destruct H, H, H17, H18.
+  eexists; intuition eauto.
+  do 2 (eapply result_same_transitive; eauto).
+  apply result_same_symmetric; auto.
+  rewrite <- H9, H12; auto.
+Qed.
+
